working on smallstep

Smallstep.v
@@ -30,3 +30,141 @@ Inductive eval : tm -> nat -> Prop :=
   where " t '\\' n " := (eval t n).
 
 Module SimpleArith1.
+
+Reserved Notation " t '=>' t' " (at level 40).
+
+Inductive step : tm -> tm -> Prop :=
+  | ST_PlusConstConst : forall n1 n2,
+    P (C n1) (C n2) => C (n1 + n2)
+  | ST_Plus1 : forall t1 t1' t2,
+    t1 => t1' ->
+    P t1 t2 => P t1' t2
+  | ST_Plus2 : forall n1 t2 t2',
+    t2 => t2' ->
+    P (C n1) t2 => P (C n1) t2'
+
+where " t '=>' t' " := (step t t').
+
+Example test_step_1 :
+  P (P (C 0) (C 3))
+    (P (C 2) (C 4))
+  =>
+  P (C (0 + 3))
+    (P (C 2) (C 4)).
+Proof. apply ST_Plus1. apply ST_PlusConstConst. Qed.
+
+Example test_step_2 :
+      P
+        (C 0)
+        (P
+          (C 2)
+          (P (C 0) (C 3)))
+      =>
+      P
+        (C 0)
+        (P
+          (C 2)
+          (C (0 + 3))).
+Proof. apply ST_Plus2. apply ST_Plus2.  apply ST_PlusConstConst. Qed.
+
+End SimpleArith1.
+
+Definition relation (X:Type) := X -> X -> Prop.
+
+Definition deterministic {X: Type} (R: relation X) :=
+  forall x y1 y2 : X, R x y1 -> R x y2 -> y1 = y2.
+
+Module SimpleArith2.
+Import SimpleArith1.
+
+Theorem step_deterministic:
+  deterministic step.
+Proof.
+  unfold deterministic. intros x y1 y2 Hy1 Hy2.
+  generalize dependent y2.
+  induction Hy1; intros y2 Hy2. 
+  - inversion Hy2.
+    + reflexivity.
+    + inversion H2.
+    + inversion H2.
+  - inversion Hy2.
+    + rewrite <- H0 in Hy1. inversion Hy1.
+    +  rewrite <- (IHHy1 t1'0).
+        reflexivity. assumption.
+    + rewrite <- H in Hy1. inversion Hy1.
+  - inversion Hy2.
+    + rewrite <- H1 in Hy1. inversion Hy1.
+    + inversion H2.
+    + rewrite <- (IHHy1 t2'0). reflexivity. assumption.
+
+Qed.
+
+End SimpleArith2.
+
+Ltac solve_by_inverts n :=
+  match goal with | H : ?T |- _ =>
+  match type of T with Prop =>
+    solve [
+      inversion H;
+      match n with S (S (?n')) => subst; solve_by_inverts (S n') end ]
+  end end.
+
+Ltac solve_by_invert :=
+  solve_by_inverts 1.
+
+Module SimpleArith3.
+Import SimpleArith1.
+
+Theorem step_deterministic_alt: deterministic step.
+Proof.
+  intros x y1 y2 Hy1 Hy2.
+  generalize dependent y2.
+  induction Hy1; intros y2 Hy2;
+    inversion Hy2; subst; try solve_by_invert.
+  - (* ST_PlusConstConst *) reflexivity.
+  - (* ST_Plus1 *)
+    apply IHHy1 in H2. rewrite H2. reflexivity.
+  - (* ST_Plus2 *)
+    apply IHHy1 in H2. rewrite H2. reflexivity.
+Qed.
+
+End SimpleArith3.
+
+Inductive value : tm -> Prop :=
+  v_const : forall n, value (C n).
+
+Reserved Notation " t '=>' t' " (at level 40).
+
+Inductive step : tm -> tm -> Prop :=
+  | ST_PlusConstConst : forall n1 n2,
+          P (C n1) (C n2)
+      => C (n1 + n2)
+  | ST_Plus1 : forall t1 t1' t2,
+        t1 => t1' ->
+        P t1 t2 => P t1' t2
+  | ST_Plus2 : forall v1 t2 t2',
+        value v1 -> (* <----- n.b. *)
+        t2 => t2' ->
+        P v1 t2 => P v1 t2'
+
+  where " t '=>' t' " := (step t t').
+
+Theorem step_deterministic : 
+  deterministic step.
+Proof.
+  unfold deterministic. intros x y1 y2 Hy1 Hy2.
+  generalize dependent y2.
+  induction Hy1; subst;  try solve_by_invert; intros y2 Hy2.
+  - inversion Hy2.
+    + reflexivity.
+    + inversion H2.
+    + inversion H3.
+  - inversion Hy2.
+    + rewrite <- H0 in Hy1. inversion Hy1.
+    + apply IHHy1 in H2. rewrite H2. reflexivity.
+    + subst. inversion H1. rewrite <- H in Hy1. inversion Hy1.
+  - inversion Hy2.
+    + rewrite <- H2 in Hy1. inversion Hy1.
+    + inversion H. subst. inversion H3.
+    + apply IHHy1 in H4. rewrite H4. reflexivity.
+Qed.
